src/OSum/logrel.v
@@ -16,7 +16,8 @@ Section logrel.
 
     (* 
     
-    persistent predicates state that the proposition P holds over the sharable parts (core) of the resource
+    persistent predicates state that the proposition P holds 
+    over the sharable parts (core) of the resource
 
     Local Program Definition uPred_persistently_def {M} (P : uPred M) : uPred M :=
         {| uPred_holds n x := P n (core x) |}.
@@ -51,66 +52,19 @@ Section logrel.
     Qed.
 
     Import uPred.
+    (* This just says that there are two locations in bijection 
+        and the second location stores a persistent predicate on values 
+        
+        using a view element for the bijection, not the authoritative element
+    *)
     Local Program Definition pointsto_def (l l' : loc) : D -n> iPropO Σ  :=
         λne P, (own name_set (gset_bij_elem l l') ∗ saved_pred_own l' (DfracDiscarded) P)%I.
     Next Obligation.
         intros l.
         red. red. intros.
-(*         eapply uPred_primitive.exist_ne.
-        red. intros s. *)
         eapply uPred_primitive.sep_ne.
         - solve_proper.
         -  eapply saved_persistent_pred_ne. exact H0.
-    Qed.
-
-(*     Local Program Definition pointsto_def (l : loc) : D -n> iPropO Σ  :=
-        λne P, (∃ (s : state), ⌜l ∈ s⌝ ∗ own name_set s  ∗ saved_pred_own l (DfracDiscarded) P)%I.
-    Next Obligation.
-        intros l.
-        red. red. intros.
-        eapply uPred_primitive.exist_ne.
-        red. intros s.
-        eapply uPred_primitive.sep_ne.
-        - solve_proper.
-        - eapply uPred_primitive.sep_ne.
-        + solve_proper.
-        + eapply saved_persistent_pred_ne. exact H0.
-    Qed.
- *)
-
-(*     Local Definition pointsto_def (l : loc)  (P : D) : iProp Σ :=
-        (∃ (s : state), ⌜l ∈ s⌝  ∗ own name_set s  ∗ saved_pred_own (encode l) (DfracDiscarded) P)%I.
- *)
-
-    (*  why do i have goals of the form  Proper (dist n ==> dist n) ?
-    where is this requirement coming from ? 
-    
-    This is how to state non,expansiveness
-        Notation NonExpansive f := (∀ n, Proper (dist n ==> dist n) f).
-
-        Notation Contractive f := (∀ n, Proper (dist_later n ==> dist n) f).
-
-
-        does being contractive prove being non expansive?
-            have f : X -> Y 
-            ne := forall (n : nat)(x y : X), x ={n}= y -> f x ={n} f y
-
-            contr := forall (n : nat)(x y : X), (forall m < n, x ={m}= y) -> f x ={n}= f y
-
-        yes, proof is here
-            https://plv.mpi-sws.org/coqdoc/iris/iris.algebra.ofe.html#contractive
-
-    *)
-
-    Lemma contrIsNe {X Y : ofe}{f : X -n> Y}(c : Contractive f) : NonExpansive f.
-    Proof.
-        eapply contractive_ne. exact c.
-    Qed.        
-
-
-    Lemma persistant_pred_ne (P : D): NonExpansive P.
-    Proof.
-        solve_proper.
     Qed.
           
     Local Notation "l @ l' ↦□ v" := (pointsto_def l l' v)
@@ -119,6 +73,7 @@ Section logrel.
     Global Instance mypointsto_persist (l l': loc)  (P : D) : Persistent (l @ l' ↦□ P).
     apply _. Qed.
 
+    (* the type of each case of the unary logical relation *)
     Definition VRelType := listO D -n> D.
 
     Program Definition interp_TVar (v : var) : VRelType := 
@@ -139,17 +94,16 @@ Section logrel.
     Solve Obligations with solve_proper.
 
     Definition interp_TCase' (interp : VRelType)(rho : listO D) : D :=
-        PersPred(fun v => (∃ l l' , ⌜v = CaseV l⌝ ∗ l @ l' ↦□ (interp rho)))%I.
+        PersPred(fun v => (∃ l l' , ⌜v = CaseV l⌝ ∗ (l @ l' ↦□ (interp rho))))%I.
 
     Local Instance interp_TCase'_ne (interp : VRelType)(rho : listO D)  : 
         NonExpansive (PersPred(fun v => (∃ l l', ⌜v = CaseV l⌝ ∗ l @ l' ↦□ (interp rho)))%I).
     Proof.        
-        eapply persistant_pred_ne.
+        solve_proper.
     Qed.
-
-
-    Check persistent_pred_car_ne val (iProp Σ) 0 (interp_TCase' _ _ )(interp_TCase' _ _ ) _ _  _ _. 
         
+    (* annoying.. The predicate for interp_TCase is non expansive...
+        But I still need to lift that for any rho... *)
     Program Definition interp_TCase (interp : VRelType) : VRelType := 
          λne rho, interp_TCase' interp rho.
     Next Obligation.
@@ -161,8 +115,6 @@ Section logrel.
         pose proof (persistent_pred_car_ne val (iProp Σ) n (interp_TCase' interp x )(interp_TCase' interp y ) ).
     Admitted.
      
-
-
     Program Definition interp_TOSum : VRelType := 
         λne rho, PersPred(fun v =>(∃ l l' v' P , ⌜v = InjV (CaseV l) v'⌝ ∗ l @ l'  ↦□ P ∗ P v'))%I.
 
@@ -198,6 +150,7 @@ Section logrel.
         intros i1. solve_proper.
     Qed.
 
+    (* The full unary logical relation  *)
     Fixpoint interp (τ : type) : listO D -n> D :=
         match τ return _ with
         | TUnit => interp_TUnit
@@ -241,72 +194,68 @@ Section logrel.
 
     Notation "⟦ τ ⟧ₑ" := (interp_expr τ).
 
-  Lemma interp_env_length Δ Γ vs : ⟦ Γ ⟧* Δ vs ⊢ ⌜length Γ = length vs⌝.
-  Proof. by iIntros "[% ?]". Qed.
+    Lemma interp_env_length Δ Γ vs : ⟦ Γ ⟧* Δ vs ⊢ ⌜length Γ = length vs⌝.
+    Proof. by iIntros "[% ?]". Qed.
 
-  Lemma interp_env_Some_l Δ Γ vs x τ :
-    Γ !! x = Some τ → ⟦ Γ ⟧* Δ vs ⊢ ∃ v, ⌜vs !! x = Some v⌝ ∧ ⟦ τ ⟧ Δ v.
-  Proof.
-    iIntros (?) "[Hlen HΓ]"; iDestruct "Hlen" as %Hlen.
-    destruct (lookup_lt_is_Some_2 vs x) as [v Hv].
-    { by rewrite -Hlen; apply lookup_lt_Some with τ. }
-    iExists v; iSplit; first done. iApply (big_sepL_elem_of with "HΓ").
-    apply elem_of_list_lookup_2 with x.
-    rewrite lookup_zip_with; by simplify_option_eq.
-  Qed.
+    Lemma interp_env_Some_l Δ Γ vs x τ :
+        Γ !! x = Some τ → ⟦ Γ ⟧* Δ vs ⊢ ∃ v, ⌜vs !! x = Some v⌝ ∧ ⟦ τ ⟧ Δ v.
+    Proof.
+        iIntros (?) "[Hlen HΓ]"; iDestruct "Hlen" as %Hlen.
+        destruct (lookup_lt_is_Some_2 vs x) as [v Hv].
+        { by rewrite -Hlen; apply lookup_lt_Some with τ. }
+        iExists v; iSplit; first done. iApply (big_sepL_elem_of with "HΓ").
+        apply elem_of_list_lookup_2 with x.
+        rewrite lookup_zip_with; by simplify_option_eq.
+    Qed.
 
-
-
-    Check upn.
-    Eval compute in upn 2 Var 9. 
-    Check ren.
-
-
+    (*  need to fix this proof *)
     Lemma interp_weaken Δ1 Π Δ2 τ :
         ⟦ τ.[upn (length Δ1) (ren (+ length Π))] ⟧ (Δ1 ++ Π ++ Δ2)
         ≡ ⟦ τ ⟧ (Δ1 ++ Δ2).
-  Proof.
-    revert Δ1 Π Δ2. induction τ=> Δ1 Π Δ2; simpl; auto; intros ?; simpl.
-    - by repeat (f_equiv; try match goal with IH : ∀ _, _ |- _ => by apply IH end).
-    - by repeat (f_equiv; try match goal with IH : ∀ _, _ |- _ => by apply IH end).
+    Proof.
+        revert Δ1 Π Δ2. induction τ=> Δ1 Π Δ2; simpl; auto; intros ?; simpl.
+        - by repeat (f_equiv; try match goal with IH : ∀ _, _ |- _ => by apply IH end).
+        - by repeat (f_equiv; try match goal with IH : ∀ _, _ |- _ => by apply IH end).
+        Admitted.
+    (*     - by repeat (f_equiv; try match goal with IH : ∀ _, _ |- _ => by apply IH end).
+        - f_equiv.
+        apply fixpoint_proper=> τi w /=.
+        by repeat (f_equiv; try match goal with IH : ∀ _, _ |- _ => by apply (IH (_ :: _)) end).
+        - rewrite iter_up; destruct lt_dec as [Hl | Hl]; simpl.
+        { by rewrite !lookup_app_l. }
+        rewrite !lookup_app_r; [|lia ..]; do 3 f_equiv; lia.
+        - by repeat (f_equiv; try match goal with IH : ∀ _, _ |- _ => by apply (IH (_ :: _)) end).
+        - by repeat (f_equiv; try match goal with IH : ∀ _, _ |- _ => by apply (IH (_ :: _)) end).
+        - by repeat (f_equiv; try match goal with IH : ∀ _, _ |- _ => by apply IH end).
+    Qed. *)
+
+    (* need to fix this proof  *)
+    Lemma interp_subst_up Δ1 Δ2 τ τ' :
+        ⟦ τ ⟧ (Δ1 ++ interp τ' Δ2 :: Δ2)
+        ≡ ⟦ τ.[upn (length Δ1) (τ' .: ids)] ⟧ (Δ1 ++ Δ2).
+    Proof.
+        revert Δ1 Δ2; induction τ=> Δ1 Δ2; simpl; auto; intros ?; simpl.
+        - by repeat (f_equiv; try match goal with IH : ∀ _, _ |- _ => by apply IH end).
+        - by repeat (f_equiv; try match goal with IH : ∀ _, _ |- _ => by apply IH end).
+        Admitted. (* by repeat (f_equiv; try match goal with IH : ∀ _, _ |- _ => by apply IH end).
+        - f_equiv.
+        apply fixpoint_proper=> τi w /=.
+        by repeat (f_equiv; try match goal with IH : ∀ _, _ |- _ => by apply (IH (_ :: _)) end).
+        - match goal with |- context [_ !! ?x] => rename x into idx end.
+        rewrite iter_up; destruct lt_dec as [Hl | Hl]; simpl.
+        { by rewrite !lookup_app_l. }
+        rewrite !lookup_app_r; [|lia ..].
+        case EQ: (idx - length Δ1) => [|n]; simpl.
+        { symmetry. asimpl. apply (interp_weaken [] Δ1 Δ2 τ'). }
+        rewrite !lookup_app_r; [|lia ..]. do 3 f_equiv. lia.
+        - by repeat (f_equiv; try match goal with IH : ∀ _, _ |- _ => by apply (IH (_ :: _)) end).
+        - by repeat (f_equiv; try match goal with IH : ∀ _, _ |- _ => by apply (IH (_ :: _)) end).
+        - by repeat (f_equiv; try match goal with IH : ∀ _, _ |- _ => by apply IH end).
+    Qed. *)
+
+    (* fix this  *)
+    Lemma interp_subst Δ2 τ τ' v : ⟦ τ ⟧ (⟦ τ' ⟧ Δ2 :: Δ2) v ≡ ⟦ τ.[τ'/] ⟧ Δ2 v.
     Admitted.
-(*     - by repeat (f_equiv; try match goal with IH : ∀ _, _ |- _ => by apply IH end).
-    - f_equiv.
-      apply fixpoint_proper=> τi w /=.
-      by repeat (f_equiv; try match goal with IH : ∀ _, _ |- _ => by apply (IH (_ :: _)) end).
-    - rewrite iter_up; destruct lt_dec as [Hl | Hl]; simpl.
-      { by rewrite !lookup_app_l. }
-      rewrite !lookup_app_r; [|lia ..]; do 3 f_equiv; lia.
-    - by repeat (f_equiv; try match goal with IH : ∀ _, _ |- _ => by apply (IH (_ :: _)) end).
-    - by repeat (f_equiv; try match goal with IH : ∀ _, _ |- _ => by apply (IH (_ :: _)) end).
-    - by repeat (f_equiv; try match goal with IH : ∀ _, _ |- _ => by apply IH end).
-  Qed. *)
-
-  Lemma interp_subst_up Δ1 Δ2 τ τ' :
-    ⟦ τ ⟧ (Δ1 ++ interp τ' Δ2 :: Δ2)
-    ≡ ⟦ τ.[upn (length Δ1) (τ' .: ids)] ⟧ (Δ1 ++ Δ2).
-  Proof.
-    revert Δ1 Δ2; induction τ=> Δ1 Δ2; simpl; auto; intros ?; simpl.
-    - by repeat (f_equiv; try match goal with IH : ∀ _, _ |- _ => by apply IH end).
-    - by repeat (f_equiv; try match goal with IH : ∀ _, _ |- _ => by apply IH end).
-    Admitted. (* by repeat (f_equiv; try match goal with IH : ∀ _, _ |- _ => by apply IH end).
-    - f_equiv.
-      apply fixpoint_proper=> τi w /=.
-      by repeat (f_equiv; try match goal with IH : ∀ _, _ |- _ => by apply (IH (_ :: _)) end).
-    - match goal with |- context [_ !! ?x] => rename x into idx end.
-      rewrite iter_up; destruct lt_dec as [Hl | Hl]; simpl.
-      { by rewrite !lookup_app_l. }
-      rewrite !lookup_app_r; [|lia ..].
-      case EQ: (idx - length Δ1) => [|n]; simpl.
-      { symmetry. asimpl. apply (interp_weaken [] Δ1 Δ2 τ'). }
-      rewrite !lookup_app_r; [|lia ..]. do 3 f_equiv. lia.
-    - by repeat (f_equiv; try match goal with IH : ∀ _, _ |- _ => by apply (IH (_ :: _)) end).
-    - by repeat (f_equiv; try match goal with IH : ∀ _, _ |- _ => by apply (IH (_ :: _)) end).
-    - by repeat (f_equiv; try match goal with IH : ∀ _, _ |- _ => by apply IH end).
-  Qed. *)
-
-  Lemma interp_subst Δ2 τ τ' v : ⟦ τ ⟧ (⟦ τ' ⟧ Δ2 :: Δ2) v ≡ ⟦ τ.[τ'/] ⟧ Δ2 v.
- Admitted.
     
 
 End logrel.
@@ -315,171 +264,3 @@ Global Typeclasses Opaque interp_env.
 Notation "⟦ τ ⟧" := (interp τ).
 Notation "⟦ τ ⟧ₑ" := (interp_expr τ).
 Notation "⟦ Γ ⟧*" := (interp_env Γ).
-
-
-(* 
-
-
-
-    (*  what is the core of our resouce ... 
-
-    Local Instance dfrac_pcore_instance : PCore dfrac := λ dq,
-        match dq with
-        | DfracOwn q ⇒ None
-        | DfracDiscarded ⇒ Some DfracDiscarded
-        | DfracBoth q ⇒ Some DfracDiscarded
-        end.
-    
-
-    what is the meaning of discarded... 
-    
-    Global Instance saved_pred_discarded_persistent γ Φ :
-        Persistent (saved_pred_own γ DfracDiscarded Φ).
-    Proof. apply _. Qed.
-
-    Do I need to say it owns it, or can it just be discarded knowledge ...
-        
-    *)
-
-    (* pure things are always persistent *)
-    Definition p1 (l : loc) : iProp Σ := (∃ (s : state), ⌜l ∈ s⌝)%I.
-    Local Instance pers_p1 (l : loc) : Persistent (p1 l).
-    Proof.
-        apply _.
-    Qed.
-
-    (*  note that
-    
-        Class CoreId {A : cmra} (x : A) := core_id : pcore x ≡ Some x.
-
-        Global Instance own_core_persistent γ a : CoreId a → Persistent (own γ a).
-        Proof. rewrite !own_eq /own_def; apply _. Qed.
-
-        recall, state := gset loc
-
-        hmm.. probably not where the instance is summoned from 
-     *)
-
-    Definition p2 : iProp Σ := (∃ (s : state), own name_set s )%I.
-    Local Instance pers_p2 : Persistent p2.
-    Proof.
-        apply _.
-    Qed.
-
-    Definition p1p2 (l : loc):  iProp Σ := (∃ (s : state), ⌜l ∈ s⌝ ∗ own name_set s )%I.
-    Local Instance pers_p1p2 (l : loc) : Persistent (p1p2 l).
-    apply _. Qed.
-
-
-    Definition p3 (l : loc)  (P : D) : iProp Σ :=  (saved_pred_own (encode l) (DfracOwn 1) P)%I.
-
-    Local Instance pers_p3 (l : loc)  (P : D) : Persistent (p3 l P).
-    Fail apply _.
-    Abort.
-   
-    Definition p3' (l : loc)  (P : D) : iProp Σ :=  (saved_pred_own (encode l) (DfracDiscarded) P)%I.
-    Local Instance pers_p3' (l : loc)  (P : D) : Persistent (p3' l P).
-    apply _. Qed.
-
-
-    (*  Global Instance saved_pred_discarded_persistent γ Φ :
-            Persistent (saved_pred_own γ DfracDiscarded Φ).
-        Proof. apply _. Qed. 
-
-
-        do the saved predicates need to be owned ...?
-
-
-        See this note on the persistent pointsto predicate from the tutorial (persistently.v)
-                    (**
-            Let us now turn to the `discarded' part. If one owns a fraction of a
-            points-to predicate, one can decide to _discard_ the fraction. This
-            means that it is no longer possible to recombine points-to predicates
-            to get the full fraction. As such, the value in the points-to
-            predicate can never be changed again – the location has become
-            read-only. We write [l ↦□ v] for a points-to predicate whose fraction
-            has been discarded. As the [□] suggests, this predicate is persistent.
-            Persistent points-to predicates are great if your program has a
-            read-only location, as it becomes trivial to give all threads access
-            to the associated points-to predicate, and it ensures that no thread
-            can sneakily update the location.
-
-            The [pointsto_persist] lemma asserts that we can update any points-to
-            predicate [l ↦{dq} v] into a persistent one [l ↦□ v].
-            *)
-    *)
-    
-
-
-    Local Instance isIt (l : loc)(P : D) : Persistent (l ↦ P).
-    Proof.
-        unfold Persistent.
-        unfold pointsto_def.
-        unfold bi_persistently.
-        eexists.
-        intros.
-
-
-        r
-        inversion  H1.
-        unfold uPred_holds. simpl. red. red.
-
-    Admitted.
-
-
-
-
-
-   Definition D := val -> iProp Σ.
-
-    Definition VRelType := list D -> D.
-
-    Definition interp_TVar (v : var) : VRelType := 
-        fun rho => (default (fun _ => True%I) (rho !! v)) .
-
-    Definition interp_TUnit : VRelType := 
-        fun rho v => ⌜v = UnitV⌝%I.
-
-    Definition interp_TInt : VRelType := 
-        fun rho v => (∃ (n : nat), ⌜v = IntV n⌝)%I.
-
-    Definition interp_TBool : VRelType := 
-        fun rho v => (∃ (b : bool), ⌜v = BoolV b⌝)%I.
-
-    Definition interp_TProd (interp1 interp2 : VRelType) : VRelType := 
-        fun rho v => (∃ v1 v2 , ⌜v = PairV v1 v2⌝  ∗ interp1 rho v1  ∗ interp2 rho v2)%I.
-
-    Definition interp_TCase (interp : VRelType) : VRelType := 
-        fun rho v => (∃ l, ⌜v = CaseV l⌝ ∗ l ↦ (interp rho))%I.
-
-    Definition interp_TOSum : VRelType := 
-        fun rho v => (∃ l v' P , ⌜v = InjV (CaseV l) v'⌝ ∗ l ↦ P ∗ P v')%I.
-
-    (* what if state is modified ? *)
-    Definition interp_TArrow (interp1 interp2 : VRelType) : VRelType := 
-        fun rho v => (□ ∀ v', interp1 rho v' →
-                        WP App (of_val v) (of_val v') {{ interp2 rho }})%I.
-
-    (* normal forall, not fresh forall
-       for fresh forall, would need to update saved predicate map? *)
-    Definition interp_TForall (interp : VRelType) : VRelType := 
-        fun rho v => (□ ∀ τi : D, WP TApp (of_val v) {{ interp (τi :: rho) }})%I.
-
-    Definition interp_TExist (interp : VRelType) : VRelType := 
-        fun rho v => (∃ (τi : D) v' ,  ⌜v = PackV v'⌝ ∗ interp (τi :: rho) v)%I.
-
-
-    Fixpoint interp (τ : type) : list D -> D :=
-        match τ return _ with
-        | TUnit => interp_TUnit
-        | TInt => interp_TInt
-        | TBool => interp_TBool
-        | TProd τ1 τ2 => interp_TProd (interp τ1) (interp τ2)
-        | TArrow τ1 τ2 => interp_TArrow (interp τ1) (interp τ2)
-        | TVar x => interp_TVar x
-        | TForall τ' => interp_TForall (interp τ')
-        | TExist τ' => interp_TExist (interp τ')
-        | TOSum => interp_TOSum
-        | TCase t => interp_TCase (interp t)
-        end.
- *)
